docs

Cslib/Foundations/Logic/Model.lean
@@ -9,20 +9,23 @@ module
 public import Cslib.Foundations.Logic.Connectives
 public import Cslib.Foundations.Logic.InferenceSystem
 public import Cslib.Logics.Modal.Basic
+public import Cslib.Logics.Propositional.NaturalDeduction.Basic
+
+/-! # Semantics for logical systems -/
 
 public section
 
 namespace Cslib.Logic
 
 /-- Objects of type `β` carry a forcing relation with the proposition type `α`. -/
-class ModelClass (α : outParam (Type*)) (β : Type*) where
+class ModelClass (α : outParam Type*) (β : Type*) where
   /-- `Forces b a` has the intended semantics "`a` is valid in the model `b`". -/
   Forces : β → α → Prop
 
 scoped notation "⊨[" b "] " a => ModelClass.Forces b a
 
 /-- Objects of type `β` carry a forcing relation worlds of type `γ` and the proposition type `α`. -/
-class ParamModelClass (α : outParam (Type*)) (β : Type*) where
+class ParamModelClass (α : outParam Type*) (β : Type*) where
   Param : β → Type*
   /-- Forcing relation associated to each parameter. -/
   ForcesAt (b : β) : (Param b) → α → Prop
@@ -33,42 +36,55 @@ instance ParamModelClass.toModelClass {α β : Type*} [ParamModelClass α β] : 
   Forces M A := ∀ w : ParamModelClass.Param M, w ⊨[M] A
 
 /-- Bundled interpretation function. -/
-structure Interp (α β : Type*) where
+class HasInterp (α : outParam Type*) (β : Type*) where
+  /-- Type carrying interpretation. -/
+  Ground : β → Type*
   /-- Interpret a proposition in a model. -/
-  interp : α → β
+  interp : (b : β) → α → Ground b
 
 /-- An `InterpModel` consists of an interpretation function, and a set specifying which
   interpretations are considered valid. -/
-structure InterpModel (α β : Type*) extends Interp α β where
+class InterpModelClass (α : outParam (Type*)) (β : Type*) extends HasInterp α β where
   /-- The set of valid interpretations. -/
-  filter : Set β
+  filter (b : β) : Set (Ground b)
 
-instance {α β : Type*} : ModelClass α (InterpModel α β) where
-  Forces M a := M.interp a ∈ M.filter
+instance InterpModelClass.instModelClass {α β : Type*} [InterpModelClass α β] : ModelClass α β where
+  Forces b a := HasInterp.interp b a ∈ filter b
 
-namespace Interp
+namespace HasInterp
 
-class AlgebraicAnd {α β : Type*} [HasAnd α] [Min β] (M : Interp α β) where
-  interp_and_eq (x y : α) : M.interp (x ∧ y) = M.interp x ⊓ M.interp y
+class AlgebraicAnd (α β : Type*) [HasInterp α β] [HasAnd α] [∀ b : β, Min (Ground b)] where
+  interp_and_eq (M : β) (x y : α) : interp M (x ∧ y) = interp M x ⊓ interp M y
 
-class AlgebraicOr {α β : Type*} [HasOr α] [Max β] (M : Interp α β) where
-  interp_or_eq (x y : α) : M.interp (x ∨ y) = M.interp x ⊔ M.interp y
+class AlgebraicOr (α β : Type*) [HasInterp α β] [HasOr α] [∀ b : β, Max (Ground b)] where
+  interp_or_eq (M : β) (x y : α) : interp M (x ∨ y) = interp M x ⊔ interp M y
 
-class AlgebraicImpl {α β : Type*} [HasImpl α] [HImp β] (M : Interp α β) where
-  interp_impl_eq (x y : α) : M.interp (x → y) = M.interp x ⇨ M.interp y
+class AlgebraicImpl (α β : Type*) [HasInterp α β] [HasImpl α] [∀ b : β, HImp (Ground b)] where
+  interp_impl_eq (M : β) (x y : α) : interp M (x → y) = interp M x ⇨ interp M y
 
-class AlgebraicNot {α β : Type*} [HasNot α] [Compl β] (M : Interp α β) where
-  interp_not_eq (x : α) : M.interp (¬ x) = (M.interp x)ᶜ
+class AlgebraicNot (α β : Type*) [HasInterp α β] [HasNot α] [∀ b : β, Compl (Ground b)] where
+  interp_not_eq (M : β) (x y : α) : interp M (¬ x) = (interp M x)ᶜ
 
-end Interp
+end HasInterp
 
 open ModelClass ParamModelClass InferenceSystem
 
-def Sound {α β S : Type*} [ModelClass α β] [InferenceSystem S α] : Prop :=
-  ∀ (A : α) (b : β) , DerivableIn S A → ⊨[b] A
+variable {α β T} [ModelClass α β] [InferenceSystem T α]
 
-def Complete {α β S : Type*} [ModelClass α β] [InferenceSystem S α] : Prop :=
-  ∀ A : α, (∀ b : β, ⊨[b] A) → DerivableIn S A
+def SoundFor (α β T) [ModelClass α β] [InferenceSystem T α] (S : Set β) : Prop :=
+  ∀ (A : α), DerivableIn T A → ∀ M ∈ S, ⊨[M] A
+
+lemma SoundFor.subset {S S' : Set β} (hS : S ⊆ S') : SoundFor α β T S' → SoundFor α β T S :=
+  fun h A hA M hM => h A hA M (hS hM)
+
+def CompleteFor (α β T : Type*) [ModelClass α β] [InferenceSystem T α] (S : Set β) : Prop :=
+  ∀ A : α, (∀ M ∈ S, ⊨[M] A) → DerivableIn T A
+
+lemma CompleteFor.supset {S S' : Set β} (hS : S ⊆ S') :
+    CompleteFor α β T S → CompleteFor α β T S' := fun h A hA => h A (fun M hM => hA M (hS hM))
+
+def IsCompleteModel (α β T) [ModelClass α β] [InferenceSystem T α] (M : β) : Prop :=
+  ∀ (A : α), (⊨[M] A) → DerivableIn T A
 
 def ParamModelClass.theory {α β : Type*} [ParamModelClass α β] {M : β} (w : Param M) : Set α :=
   {A : α | w ⊨[M] A}
@@ -93,6 +109,62 @@ example {World Atom : Type*} (S : Set (Model World Atom)) :
   simp [ModelClass.logic]
   rfl
 
+example {World Atom : Type*} (m : Model World Atom) (w : World) :
+    theory m w = ParamModelClass.theory (M := m.toBundledModel) w := by
+  simp [theory, ParamModelClass.theory]
+  rfl
+
 end Modal
+
+namespace PL
+
+variable {Atom : Type*}
+
+instance : HasAnd (Proposition Atom) := ⟨Proposition.and⟩
+instance : HasOr (Proposition Atom) := ⟨Proposition.or⟩
+instance : HasImpl (Proposition Atom) := ⟨Proposition.impl⟩
+instance [Bot Atom] : HasNot (Proposition Atom) := ⟨Proposition.neg⟩
+
+structure HeytingModel (Atom : Type*) where
+  H : Type*
+  [inst : GeneralizedHeytingAlgebra H]
+  v : Atom → H
+
+instance (M : HeytingModel Atom) : GeneralizedHeytingAlgebra M.H := M.inst
+
+def HeytingModel.interp (M : HeytingModel Atom) : Proposition Atom → M.H
+  | Proposition.atom x => M.v x
+  | Proposition.and A B => M.interp A ⊓ M.interp B
+  | Proposition.or A B => M.interp A ⊔ M.interp B
+  | Proposition.impl A B => M.interp A ⇨ M.interp B
+
+instance : InterpModelClass (Proposition Atom) (HeytingModel Atom) where
+  Ground M := M.H
+  interp := HeytingModel.interp
+  filter _ := {⊤}
+
+instance (M : HeytingModel Atom) : GeneralizedHeytingAlgebra (HasInterp.Ground M) := M.inst
+
+instance : HasInterp.AlgebraicAnd (Proposition Atom) (HeytingModel Atom) where
+  interp_and_eq _ _ _ := rfl
+
+instance : HasInterp.AlgebraicOr (Proposition Atom) (HeytingModel Atom) where
+  interp_or_eq _ _ _ := rfl
+
+instance : HasInterp.AlgebraicImpl (Proposition Atom) (HeytingModel Atom) where
+  interp_impl_eq _ _ _ := rfl
+
+theorem HeytingModel.sound [DecidableEq Atom] {T : Theory Atom} :
+    SoundFor (Proposition Atom) (HeytingModel Atom) T {M | ∀ A ∈ T, interp M A = ⊤} :=
+  sorry -- i have this in a branch
+
+def Theory.lindenbaum [DecidableEq Atom] (T : Theory Atom) : HeytingModel Atom :=
+  sorry -- usual Heyting-algebra of propositions modulo equivalence
+
+theorem Theory.lindenbaum_complete [DecidableEq Atom] {T : Theory Atom} :
+    IsCompleteModel (Proposition Atom) (HeytingModel Atom) T T.lindenbaum :=
+  sorry -- also in a branch
+
+end PL
 
 end Cslib.Logic
